initAddrspace verifies and preserves validPageDB. Partial implementation of initDispatcher and allocatePage. See notes Verifying initAddrspace required the addition of pageDbEntriesValidRefs to validPageDb. An ongoing issue seems to be that updating one pageDB entry may make other pages invalid, so proving that validity is preserved by updates is difficult. validPageDb has been partially refactored to make debuggint this issue easier.

verified/pagedb.dfy
@@ -32,40 +32,88 @@ datatype PageDbEntry
 
 type PageDb = imap<PageNr, PageDbEntry>
 
+predicate wellFormedPageDb(d: PageDb)
+{
+    forall n :: validPageNr(n) <==> n in d
+}
+
 predicate validPageDb(d: PageDb)
 {
-    // the domain of d must equal all valid pages
-    forall n :: validPageNr(n) <==> n in d
-        // all entries are valid
-        && forall n :: n in d ==> validPageDbEntry(d, n)
+    wellFormedPageDb(d)
+    && pageDbEntriesAddrspacesOk(d)
+    && pageDbEntriesValid(d)
+    && pageDbEntriesValidRefs(d)
+}
+
+predicate pageDbEntriesAddrspacesOk(d:PageDb)
+    requires wellFormedPageDb(d)
+{
+    forall n :: n in d && d[n].PageDbEntryTyped? ==> pageDbEntryAddrspacesOk(d, n)
+}
+
+predicate pageDbEntriesValid(d:PageDb)
+    requires wellFormedPageDb(d)
+    requires pageDbEntriesAddrspacesOk(d)
+{
+    forall n :: n in d ==> validPageDbEntry(d, n)
+}
+
+predicate pageDbEntriesValidRefs(d: PageDb)
+{
+    forall n :: n in d && d[n].PageDbEntryTyped? ==> 
+        pageDbEntryValidRefs(d, n)
 }
 
 predicate validPageDbEntry(d: PageDb, n: PageNr)
     requires n in d
 {
     var e := d[n];
-    e.PageDbEntryFree? || (e.PageDbEntryTyped? && validPageDbEntryTyped(d, n))
+    e.PageDbEntryFree? || (e.PageDbEntryTyped? &&
+        pageDbEntryAddrspacesOk(d, n) &&
+        validPageDbEntryTyped(d, n))
+}
+
+predicate pageDbEntryAddrspacesOk(d: PageDb, n: PageNr)
+    requires n in d && d[n].PageDbEntryTyped?
+{
+    var e := d[n];
+    e.addrspace in d
+    && d[e.addrspace].PageDbEntryTyped?
+    && d[e.addrspace].entry.Addrspace?
 }
 
 predicate validPageDbEntryTyped(d: PageDb, n: PageNr)
     requires n in d && d[n].PageDbEntryTyped?
+    requires pageDbEntryAddrspacesOk(d, n)
 {
     var e := d[n];
-    // check that the addrspace ref is to a page of the right type
-    // (we'll check its validity when we check that entry)
-    e.addrspace in d && (
-    var addrspace := d[e.addrspace];
-    addrspace.PageDbEntryTyped? && addrspace.entry.Addrspace?
-    // type-specific checks
-    && (
-        var addrspaceIsStopped := addrspace.entry.state == StoppedState;
-        (e.entry.Addrspace? && wellFormedAddrspace(d, n))
-        || (e.entry.L1PTable? && (addrspaceIsStopped || validL1PTable(d, n)))
-        || (e.entry.L2PTable? && (addrspaceIsStopped || validL2PTable(d, n)))
-        || (e.entry.Dispatcher?)
-        || (e.entry.DataPage?)
-    ))
+    var addrspaceIsStopped := d[e.addrspace].entry.state == StoppedState;
+    (e.entry.Addrspace? && wellFormedAddrspace(d, n))
+    || (e.entry.L1PTable? && (addrspaceIsStopped || validL1PTable(d, n)))
+    || (e.entry.L2PTable? && (addrspaceIsStopped || validL2PTable(d, n)))
+    || (e.entry.Dispatcher? )
+    || (e.entry.DataPage? )
 }
+
+// Free pages and non-addrspace entries should have a refcount of 0
+predicate pageDbEntryValidRefs(d: PageDb, n: PageNr)
+    requires n in d
+{
+    var e := d[n];
+    (e.PageDbEntryTyped? && e.entry.Addrspace?) ||
+        forall m : PageNr :: validPageNr(m) ==>
+            addrspaceRefCount(d, n) == 0
+}
+
+// predicate lemma_validPageDBImpliesWellFormedAddrspaces(d: PageDb, n: PageNr)
+//     requires validPageDb(d)
+//     requires wellFormedPageDb(d)
+//     requires validPageNr(n)
+//     requires d[n].PageDbEntryTyped? && d[n].entry.Addrspace?
+//     ensures lemma_validPageDBImpliesWellFormedAddrspaces(d, n)
+// {
+//     wellFormedAddrspace(d, n) && validAddrspace(d, n)
+// }
 
 predicate validL1PTable(d: PageDb, n: PageNr)
     requires n in d && d[n].PageDbEntryTyped? && d[n].entry.L1PTable?
@@ -110,29 +158,31 @@ predicate validL2PTE(d: PageDb, addrspace: PageNr, pte: PageNr)
         && d[pte].entry.DataPage?
 }
 
-predicate validAddrspace(d: PageDb, n: PageNr)
+predicate wellFormedAddrspace(d: PageDb, n: PageNr)
     { n in d && d[n].PageDbEntryTyped? && d[n].entry.Addrspace? }
    
-predicate wellFormedAddrspace(d: PageDb, n: PageNr)
-    requires validAddrspace(d, n);
+predicate validAddrspace(d: PageDb, n: PageNr)
+    requires wellFormedAddrspace(d, n);
 {
     var a := d[n].entry;
     // valid L1PT page
-    validPageNr(a.l1ptnr)
+    wellFormedAddrspace(d, n)
+        && validPageNr(a.l1ptnr)
         && a.l1ptnr in d
         && d[a.l1ptnr].PageDbEntryTyped?
         && d[a.l1ptnr].entry.L1PTable?
         // correct refcount
-        && a.refcount == addrspaceRefcount(d, n)
+        && a.refcount == addrspaceRefCount(d, n)
 }
 
 // returns the number of references to an addrspace page with the given index
-function addrspaceRefcount(d: PageDb, addrspacePageNr: PageNr): nat
+function addrspaceRefCount(d: PageDb, addrspacePageNr: PageNr): nat
     requires addrspacePageNr in d
 {
     // XXX: inlined validPageNr(n) to help dafny see that this set is bounded
     |(set n | 0 <= n < KEVLAR_SECURE_NPAGES() && n in d
-        && d[n].PageDbEntryTyped? && n != addrspacePageNr
+        && d[n].PageDbEntryTyped?
+        && n != addrspacePageNr
         && d[n].addrspace == addrspacePageNr)|
 }
 
@@ -141,3 +191,21 @@ function initialPageDb(): PageDb
 {
   imap n: PageNr | validPageNr(n) :: PageDbEntryFree
 }
+
+//-----------------------------------------------------------------------------
+// PageDB Updates
+//-----------------------------------------------------------------------------
+// lemma updatesToFreeEntriesPreserveValidity(pageDbIn: PageDb, pageDbOut: PageDb, p:PageNr)
+//     requires validPageDb(pageDbIn);
+//     requires wellFormedPageDb(pageDbOut);
+//     requires validPageNr(p);
+//     requires pageDbIn[p].PageDbEntryFree?
+//     requires pageDbOut[p].PageDbEntryTyped?
+//     requires !pageDbOut[p].entry.Addrspace?
+//     requires forall n :: n in pageDbIn && n != p &&
+//         n != pageDbOut[p].addrspace ==> pageDbOut[n] == pageDbIn[n]
+//     ensures  forall n :: n in pageDbIn && n != p &&
+//         n != pageDbOut[p].addrspace ==> validPageDbEntry(pageDbOut, n)
+// {
+// }
+
